theories/iris_examples.v
@@ -1,0 +1,33 @@
+
+From mathcomp Require Import ssreflect ssrbool eqtype seq.
+
+Set Implicit Arguments.
+Unset Strict Implicit.
+Unset Printing Implicit Defensive.
+
+From stdpp Require Import gmap strings.
+From iris.algebra Require Import auth.
+From iris.bi.lib Require Import fractional.
+From iris.proofmode Require Import tactics.
+From iris.base_logic.lib Require Import gen_heap proph_map gen_inv_heap.
+From iris.program_logic Require Import weakestpre total_weakestpre.
+From iris.program_logic Require Export language lifting.
+
+Require Export common operations_iris datatypes_iris datatypes_properties_iris properties_iris.
+Require Import iris_locations iris.
+
+Definition instance1 := 1.
+Definition instance2 := 2.
+
+Definition store11 := list_byte_of_string "store11".
+Definition store42 := list_byte_of_string "store42".
+
+Notation "A ;;; B" := (HE_seq A B) (at level 2).
+Notation "A ::= B" := (HE_setglobal A B) (at level 5).
+
+Definition Program1 :=
+  10 ::= 
+  10 ::= (HE_new_rec [::(store11, )])
+
+Lemma example1:
+  
